
#### Avansert: Utføre formell omforming av brøk,  Øveoppgaver

1. Regn ut.

   a. $\frac{3}{2}\left( 7 + \frac{3\  + \ \frac{1}{5}}{\frac{2}{3}} \right) - 1$
   \
   b. $\frac{\left( \frac{4}{7}\  \cdot \ 2\ \frac{3}{5} \right)\  - \ 3}{\frac{2}{3}} + 8$
   \
   c. $\frac{\frac{4}{3}\  + \ 5}{\frac{3}{4}\  + \ \frac{3}{5}} + \frac{7}{2}\left( 1 - \frac{8}{3} \right)$
   \
   d. $\left( \frac{\left( 2\ \ :\ \frac{2}{3} \right)\  \cdot \ \frac{3}{2}}{1\  + \ \frac{3}{2}} - \frac{4}{5} \right) \cdot (\frac{4}{5} - 2)$
   \
   e. $\frac{\frac{-3}{4}+\frac{1}{3}}{\frac{1}{6}}+ 2(\frac{5}{3}-\frac{2}{6})$
   \
   f. $\left(\frac{\left(\frac{1}{7}-\frac{1}{2}\right)}{\left(\frac{1}{2}+\frac{3}{7}\right)}\right)+ 2(\frac{1}{2}-\frac{8}{26})$
   \
   g. $\left(\frac{(2:\frac{1}{6})\cdot 5}{2-\frac{4}{3}}- 10\right)\cdot (\frac{5}{8}-\frac{1}{2})$

##### Løsningsforslag

1. \
a.
$$
\begin{aligned}
\frac{3}{2}\left( 7 + \frac{16}{5} \cdot \frac{3}{2} \right) - 1
& = \frac{3}{2} \cdot \frac{35 + 24}{5} - 1
\\
& = \frac{177}{10} - \frac{10}{10}
\\
& = \frac{167}{10}
\end{aligned}
$$
b.
$$
\begin{aligned}
\frac{4 \cdot 13-105}{7 \cdot 5} \cdot \frac{3}{2} + 8
&
= {\frac{53}{7 \cdot 5} \cdot \frac{3}{2} + 8}
\\
&
= {\frac{-159\cdot 3}{7\cdot 5\cdot 2} + \frac{560}{7\cdot 5\cdot 2}}
\\
& = \frac{401}{70}
\end{aligned}
$$
c.
$$
\begin{aligned}
\frac{19}{3} \cdot \frac{20}{27} + \frac{7}{2} \cdot \left( - \frac{5}{3} \right)
 &
 =\frac{380}{81} - \frac{35}{6}
\\
&= \frac{760}{162} - \frac{945}{162}
\\
& = - \frac{185}{162}
\end{aligned}
$$
d.
$$
\begin{aligned}
{\left( \left( 2 \cdot \frac{3}{2} \cdot \frac{3}{2} \right) \cdot \frac{2}{5} - \frac{4}{5} \right) \cdot \left( - \frac{6}{5} \right)
}
&
= {\left( \frac{9}{5} - \frac{4}{5} \right) \cdot \left( - \frac{6}{5} \right)
}
\\
& = {- \frac{6}{5}}
\end{aligned}
$$
e.
$$
\begin{aligned}
\frac{\frac{-3}{4}+\frac{1}{3}}{\frac{1}{6}}+ 2(\frac{5}{3}-\frac{2}{6}) 
& = \frac{\frac{-9+4}{12}}{\frac{1}{6}}+2(\frac{10-2}{6})
\\
& =
\frac{\frac{-5}{12}\cdot \frac{6}{1}}{\frac{1}{6}\frac{6}{1}}+2\cdot \frac{8}{6}
\\
& = 
\frac{-5}{2}+\frac{16}{6} = \frac{-15+16}{6} = \frac{1}{6}
\end{aligned}
$$
f.
$$
\begin{aligned}
\left(\frac{\left(\frac{1}{7}-\frac{1}{2}\right)}{\left(\frac{1}{2}+\frac{3}{7}\right)}\right)+ 2(\frac{1}{2}-\frac{8}{26}) 
& =
\frac{\frac{2-7}{14}}{\frac{7+6}{14}} +2(\frac{13-8}{26})
\\
& =
\frac{\frac{-5}{14}\cdot 14}{\frac{13}{14}\cdot 14} + \frac{5}{13}
\\
& = 
\frac{-5}{13}+\frac{5}{13} = 0
\end{aligned}
$$
g.
$$
\begin{aligned}
\left(\frac{(2:\frac{1}{6})\cdot 5}{2-\frac{4}{3}}- 10\right)\cdot (\frac{5}{8}-\frac{1}{2})
& =
\left(\frac{12\cdot 5}{\frac{6-4}{3}} - 10 \right)\cdot(\frac{5-4}{8})
\\
& = 
\left(\frac{12\cdot 5\cdot 3}{\frac{2}{3}\cdot 3} - 10\right)\cdot \frac{1}{8}
\\
& =
\left(\frac{180}{2}- 10 \right)\cdot \frac{1}{8} = 80\cdot \frac{1}{8} = 10
\end{aligned}
$$


#### Avansert: Utføre formell omforming av brøk,  24.04

Regn ut.

a. $((\frac{4}{5} + \frac{1}{\frac{7}{3}}) \frac{1}{43}) \cdot 7 + \frac{4}{5}$
b. $\frac{1}{2} - \frac{\frac{4}{11}((\frac{8}{6} : \frac{1}{3}) + \frac{2}{5})}{\frac{4}{2,5}}$

##### Vurderingskriterier

1, -1/2


#### Avansert: Utføre formell omforming av brøk,  17.04.23

Regn ut.

a. $\frac{3}{2}(2 + \frac{2}{3} - \frac{3 + \frac{1}{5}}{\frac{3}{2}}) -1$
b. $\frac{(\frac{4}{7} \cdot (2 + \frac{4}{5})) - \frac{3}{5}}{\frac{2}{3}} + \frac{1}{2}$

##### Vurderingskriterier

-1/5 og 2.


